monomorphize extern_ptr

steel/Zeta.Steel.ExternalPtr.fst
@@ -1,11 +1,11 @@
 module Zeta.Steel.ExternalPtr
 
-let extern_ptr a = A.array a
+let extern_ptr = A.array U8.t
 
 let gtake p = p
 
 assume
-val enclave_api_validate (#a: Type) (x:A.array a) (n: U32.t) : Pure bool
+val enclave_api_validate (x:A.array U8.t) (n: U32.t) : Pure bool
   (requires True)
   (ensures (fun b -> b == true ==> U32.v n == A.length x))
 
